make chacha20poly1305 spec more high-level

code/chacha20poly1305/Hacl.Impl.Chacha20Poly1305.PolyCore.fst
@@ -11,7 +11,6 @@ open Lib.Buffer
 open Hacl.Impl.Poly1305.Fields
 open Hacl.Spec.Poly1305.Equiv
 
-module SpecPolyVec = Hacl.Spec.Poly1305.Vec
 module SpecPoly = Spec.Poly1305
 module Spec = Spec.Chacha20Poly1305
 module Poly = Hacl.Impl.Poly1305
@@ -20,43 +19,46 @@ inline_for_extraction noextract
 let poly1305_padded_st (w:field_spec) =
     ctx:Poly.poly1305_ctx w
   -> len:size_t
-  -> text:lbuffer uint8 len
-  -> tmp:lbuffer uint8 16ul ->
+  -> text:lbuffer uint8 len ->
   Stack unit
     (requires fun h ->
-      live h ctx /\ live h text /\ live h tmp /\
-      disjoint ctx text /\ disjoint ctx tmp /\ disjoint text tmp /\
+      live h ctx /\ live h text /\ disjoint ctx text /\
       Poly.state_inv_t h ctx)
     (ensures fun h0 _ h1 ->
-      modifies (loc tmp |+| loc ctx) h0 h1 /\
+      modifies (loc ctx) h0 h1 /\
       Poly.state_inv_t h1 ctx /\
       // Additional framing for r_elem
       Poly.as_get_r h0 ctx == Poly.as_get_r h1 ctx /\
       // Functional spec
       Poly.as_get_acc h1 ctx ==
-      Spec.poly1305_padded
-        (Poly.as_get_r h0 ctx)
-        (v len)
-        (as_seq h0 text)
-        (as_seq h0 tmp)
-        (Poly.as_get_acc h0 ctx))
+      Spec.poly1305_padded (Poly.as_get_r h0 ctx) (as_seq h0 text) (Poly.as_get_acc h0 ctx))
+
+#set-options "--z3rlimit 50 --max_fuel 0 --max_ifuel 1"
 
 inline_for_extraction noextract
 val poly1305_padded_: #w:field_spec -> poly1305_padded_st w
-let poly1305_padded_ #w ctx len text tmp =
+let poly1305_padded_ #w ctx len text =
+  let h0 = ST.get () in
+  push_frame ();
+  let h1 = ST.get () in
+  Poly.reveal_ctx_inv ctx h0 h1;
   let n = len /. 16ul in
   let r = len %. 16ul in
   let blocks = sub text 0ul (n *! 16ul) in
   let rem = sub text (n *! 16ul) r in // the extra part of the input data
-  let h0 = ST.get() in
   Poly.poly1305_update #w ctx (n *! 16ul) blocks;
-  let h1 = ST.get() in
-  poly_eq_lemma #(width w) (as_seq h0 blocks) (Poly.as_get_acc h0 ctx) (Poly.as_get_r h0 ctx);
+  let h2 = ST.get () in
+  poly_eq_lemma #(width w) (as_seq h1 blocks) (Poly.as_get_acc h1 ctx) (Poly.as_get_r h1 ctx);
+  let tmp = create 16ul (u8 0) in
   update_sub tmp 0ul r rem;
-  let h2 = ST.get() in
-  Poly.reveal_ctx_inv ctx h1 h2;
+  let h3 = ST.get() in
+  Poly.reveal_ctx_inv ctx h2 h3;
   if r >. 0ul then
-    Poly.poly1305_update1 ctx tmp
+    Poly.poly1305_update1 ctx tmp;
+  let h4 = ST.get () in
+  pop_frame();
+  let h5 = ST.get () in
+  Poly.reveal_ctx_inv ctx h4 h5
 
 [@CInline]
 let poly1305_padded_32 : poly1305_padded_st M32 = poly1305_padded_
