code/chacha20poly1305/Hacl.Chacha20Poly1305_128.fst
@@ -1,6 +1,6 @@
 module Hacl.Chacha20Poly1305_128
 
-open Hacl.Chacha20Poly1305
+open Hacl.Impl.Chacha20Poly1305
 open Hacl.Impl.Poly1305.Fields
 
 #set-options "--z3rlimit 50 --max_fuel 0 --max_ifuel 0"
