code/chacha20poly1305/Hacl.Impl.Chacha20Poly1305.fst
@@ -1,0 +1,181 @@
+module Hacl.Impl.Chacha20Poly1305
+
+module ST = FStar.HyperStack.ST
+open FStar.HyperStack.All
+open FStar.HyperStack
+open FStar.Mul
+
+open Lib.IntTypes
+open Lib.Buffer
+open Lib.ByteBuffer
+
+open Hacl.Impl.Chacha20Poly1305.PolyCore
+open Hacl.Impl.Poly1305.Fields
+
+module LSeq = Lib.Sequence
+module BSeq = Lib.ByteSequence
+
+module Spec = Spec.Chacha20Poly1305
+module Chacha = Hacl.Impl.Chacha20
+module ChachaCore = Hacl.Impl.Chacha20.Core32
+
+module SpecPoly = Spec.Poly1305
+module Poly = Hacl.Impl.Poly1305
+
+#set-options "--z3rlimit 50 --max_fuel 0 --max_ifuel 1"
+
+val derive_key:
+    k:lbuffer uint8 32ul
+  -> n:lbuffer uint8 12ul
+  -> out:lbuffer uint8 64ul ->
+  Stack unit
+    (requires fun h -> live h k /\ live h out /\ live h n /\
+      disjoint k out /\ disjoint n out)
+    (ensures fun h0 _ h1 -> modifies (loc out) h0 h1 /\
+      as_seq h1 out == Spec.Chacha20.chacha20_key_block0 (as_seq h0 k) (as_seq h0 n))
+let derive_key k n out =
+  push_frame();
+  let ctx = ChachaCore.create_state () in
+  let ctx_core = ChachaCore.create_state () in
+  Chacha.chacha20_init ctx k n 0ul;
+  Chacha.chacha20_core ctx_core ctx 0ul;
+  ChachaCore.store_state out ctx_core;
+  pop_frame()
+
+#reset-options "--z3rlimit 100 --max_fuel 1 --max_ifuel 1 --using_facts_from '* -FStar.Seq'"
+
+inline_for_extraction noextract
+val poly1305_do_:
+    #w:field_spec
+  -> k:lbuffer uint8 32ul // key
+  -> aadlen:size_t
+  -> aad:lbuffer uint8 aadlen // authenticated additional data
+  -> mlen:size_t
+  -> m:lbuffer uint8 mlen // plaintext
+  -> out:lbuffer uint8 16ul // output: tag
+  -> ctx:Poly.poly1305_ctx w
+  -> block:lbuffer uint8 16ul ->
+  Stack unit
+    (requires fun h ->
+      live h k /\ live h aad /\ live h m /\ live h out /\ live h ctx /\ live h block /\
+      disjoint k out /\
+      disjoint ctx k /\ disjoint ctx aad /\ disjoint ctx m /\ disjoint ctx out /\ disjoint ctx block /\
+      disjoint block k /\ disjoint block aad /\ disjoint block m /\ disjoint block out)
+    (ensures fun h0 _ h1 ->
+      modifies (loc out |+| loc ctx |+| loc block) h0 h1 /\
+      as_seq h1 out == Spec.poly1305_do (as_seq h0 k) (as_seq h0 m) (as_seq h0 aad))
+let poly1305_do_ #w k aadlen aad mlen m out ctx block =
+  Poly.poly1305_init ctx k;
+  poly1305_padded ctx aadlen aad;
+  poly1305_padded ctx mlen m;
+  let h0 = ST.get () in
+  update_sub_f h0 block 0ul 8ul
+    (fun h -> BSeq.uint_to_bytes_le #U64 (to_u64 aadlen))
+    (fun _ -> uint_to_bytes_le (sub block 0ul 8ul) (to_u64 aadlen));
+  let h1 = ST.get () in
+  assert (LSeq.sub (as_seq h1 block) 0 8 == BSeq.uint_to_bytes_le #U64 (to_u64 aadlen));
+  Poly.reveal_ctx_inv ctx h0 h1;
+  update_sub_f h1 block 8ul 8ul
+    (fun h -> BSeq.uint_to_bytes_le #U64 (to_u64 mlen))
+    (fun _ -> uint_to_bytes_le (sub block 8ul 8ul) (to_u64 mlen));
+  let h2 = ST.get () in
+  assert (LSeq.sub (as_seq h2 block) 8 8 == BSeq.uint_to_bytes_le #U64 (to_u64 mlen));
+  LSeq.eq_intro (LSeq.sub (as_seq h2 block) 0 8) (BSeq.uint_to_bytes_le #U64 (to_u64 aadlen));
+  LSeq.lemma_concat2 8 (BSeq.uint_to_bytes_le #U64 (to_u64 aadlen)) 8 (BSeq.uint_to_bytes_le #U64 (to_u64 mlen)) (as_seq h2 block);
+  assert (as_seq h2 block == LSeq.concat (BSeq.uint_to_bytes_le #U64 (to_u64 aadlen)) (BSeq.uint_to_bytes_le #U64 (to_u64 mlen)));
+  Poly.reveal_ctx_inv ctx h1 h2;
+  Poly.poly1305_update1 ctx block;
+  Poly.poly1305_finish out k ctx
+
+// Implements the actual poly1305_do operation
+inline_for_extraction noextract
+let poly1305_do_core_st (w:field_spec) =
+    k:lbuffer uint8 32ul // key
+  -> aadlen:size_t
+  -> aad:lbuffer uint8 aadlen // authenticated additional data
+  -> mlen:size_t
+  -> m:lbuffer uint8 mlen // plaintext
+  -> out:lbuffer uint8 16ul -> // output: tag
+  Stack unit
+    (requires fun h ->
+      live h k /\ live h aad /\ live h m /\ live h out /\
+      disjoint k out)
+    (ensures fun h0 _ h1 ->
+      modifies (loc out) h0 h1 /\
+      as_seq h1 out ==
+      Spec.poly1305_do (as_seq h0 k) (as_seq h0 m) (as_seq h0 aad))
+
+inline_for_extraction noextract
+val poly1305_do_core: #w:field_spec -> poly1305_do_core_st w
+let poly1305_do_core #w k aadlen aad mlen m out =
+  push_frame();
+  let ctx = create (nlimb w +! precomplen w) (limb_zero w) in
+  let block = create 16ul (u8 0) in
+  poly1305_do_ k aadlen aad mlen m out ctx block;
+  pop_frame()
+
+[@CInline]
+let poly1305_do_32 : poly1305_do_core_st M32 = poly1305_do_core
+[@CInline]
+let poly1305_do_128 : poly1305_do_core_st M128 = poly1305_do_core
+[@CInline]
+let poly1305_do_256 : poly1305_do_core_st M256 = poly1305_do_core
+
+inline_for_extraction noextract
+val poly1305_do: #w:field_spec -> poly1305_do_core_st w
+let poly1305_do #w =
+  match w with
+  | M32 -> poly1305_do_32
+  | M128 -> poly1305_do_128
+  | M256 -> poly1305_do_256
+
+// Derives the key, and then perform poly1305
+inline_for_extraction noextract
+val derive_key_poly1305_do:
+    #w:field_spec
+  -> k:lbuffer uint8 32ul
+  -> n:lbuffer uint8 12ul
+  -> aadlen:size_t
+  -> aad:lbuffer uint8 aadlen
+  -> mlen:size_t
+  -> m:lbuffer uint8 mlen
+  -> out:lbuffer uint8 16ul ->
+  Stack unit
+    (requires fun h ->
+      live h k /\ live h n /\ live h aad /\ live h m /\ live h out)
+    (ensures  fun h0 _ h1 -> modifies (loc out) h0 h1 /\
+     (let key = Spec.Chacha20.chacha20_key_block0 (as_seq h0 k) (as_seq h0 n) in
+      let poly_k = LSeq.sub key 0 32 in
+      as_seq h1 out == Spec.poly1305_do poly_k (as_seq h0 m) (as_seq h0 aad)))
+let derive_key_poly1305_do #w k n aadlen aad mlen m out =
+  push_frame ();
+  // Create a new buffer to derive the key
+  let tmp = create 64ul (u8 0) in
+  derive_key k n tmp;
+  // The derived key should only be the first 32 bytes
+  let key = sub tmp 0ul 32ul in
+  poly1305_do #w key aadlen aad mlen m out;
+  pop_frame()
+
+let aead_encrypt #w k n aadlen aad mlen m cipher mac =
+  Chacha.chacha20_encrypt mlen cipher m k n 1ul;
+  derive_key_poly1305_do #w k n aadlen aad mlen cipher mac
+
+let aead_decrypt #w k n aadlen aad mlen m cipher mac =
+  push_frame();
+  let h0 = get() in
+  // Create a buffer to store the temporary mac
+  let computed_mac = create 16ul (u8 0) in
+  // Compute the expected mac using Poly1305
+  derive_key_poly1305_do #w k n aadlen aad mlen cipher computed_mac;
+  let h1 = get() in
+  let res =
+    if lbytes_eq computed_mac mac then (
+      assert (Lib.ByteSequence.lbytes_eq (as_seq h1 computed_mac) (as_seq h1 mac));
+      // If the computed mac matches the mac given, decrypt the ciphertext and return 0
+      Chacha.chacha20_encrypt mlen m cipher k n 1ul;
+      0ul
+    ) else 1ul // Macs do not agree, do not decrypt
+  in
+  pop_frame();
+  res
