code/poly1305/Hacl.Impl.Poly1305.fsti
@@ -26,7 +26,7 @@ val state_inv_t: #s:field_spec -> h:mem -> ctx:poly1305_ctx s -> Type0
 // If the ctx is not modified, all the components and invariants are preserved
 val reveal_ctx_inv: #s:field_spec -> ctx:poly1305_ctx s -> h0:mem -> h1:mem ->
   Lemma
-    (requires Seq.equal (as_seq h0 ctx) (as_seq h1 ctx) /\ state_inv_t h0 ctx)
+    (requires as_seq h0 ctx == as_seq h1 ctx /\ state_inv_t h0 ctx)
     (ensures
       as_get_r h0 ctx == as_get_r h1 ctx /\
       as_get_acc h0 ctx == as_get_acc h1 ctx /\
